Initial messing with oklib

OkLib.v
@@ -2,6 +2,7 @@ Require Import Setoid.
 Require Export Shared.
 Require Export PermutLib.
 Require Export PPermutLib.
+Require Export FSetLib.
 
 Open Scope permut_scope.
 
@@ -53,16 +54,6 @@ Proof. intros; rewrite flat_map_app; simpl; rew_app; auto. Qed.
 End FlatMapProp.
 
 End Definitions.
-
-Definition fst_ {A} {B} (p: A * B) :=
-  match p with
-  | (x, y) => x
-  end.
-
-Definition snd_ {A} {B} (p:A * B) :=
-  match p with
-  | (x, y) => y
-  end.
 
 Hint Rewrite flat_map_nil flat_map_cons flat_map_app flat_map_last :
   rew_flat_map.
@@ -127,36 +118,6 @@ forall x y,
 induction x; intros.
 rew_app; simpl; rewrite from_list_nil; rewrite union_empty_l; auto.
 rew_app; destruct a; simpl; rewrite IHx; rewrite union_assoc; auto.
-Qed.
-
-Lemma from_list_map:
-forall A B (l: list (A * B)) l',
-  l *=* l' ->
-  from_list (map fst_ l) = from_list (map fst_ l').
-intros A B; induction l; intros.
-apply permut_nil_eq in H; subst; auto.
-assert (a :: l *=* l') by auto;
-apply permut_split_head in H; destruct H as (hd', (tl', H)); subst.
-assert (from_list (map fst_ l) = from_list (map fst_ (hd' ++ tl'))).
-  apply IHl; apply permut_cons_inv with (a:=a); rewrite H0; permut_simpl.
-  destruct a; rew_map; simpl; rewrite from_list_cons; rewrite H.
-  rewrite map_app; repeat rewrite from_list_app; rewrite from_list_cons.
-  rewrite union_comm_assoc; auto.
-Qed.
-
-Lemma from_list_Mem:
-forall A U (x:A), Mem x U <-> x \in from_list U.
-intro A; induction U; split; intros.
-rewrite Mem_nil_eq in H; contradiction.
-rewrite from_list_nil in H; apply notin_empty in H; contradiction.
-rewrite Mem_cons_eq in H; destruct H; subst; rewrite from_list_cons;
-rewrite in_union.
-  left; rewrite in_singleton; auto.
-  right; eapply IHU; auto.
-rewrite Mem_cons_eq; rewrite from_list_cons in H; rewrite in_union in H;
-destruct H; subst.
-  left; rewrite in_singleton in H; subst; auto.
-  right; eapply IHU; auto.
 Qed.
 
 Add Morphism used_t_vars: PPermut_used_t.
