FSetLib.v
@@ -1,0 +1,44 @@
+(* Rename to fsetpermut or move to permutlib *)
+Require Export PermutLib.
+
+Open Scope permut_scope.
+
+Definition fst_ {A} {B} (p: A * B) :=
+  match p with
+  | (x, y) => x
+  end.
+
+Definition snd_ {A} {B} (p:A * B) :=
+  match p with
+  | (x, y) => y
+  end.
+
+Lemma from_list_map:
+forall A B (l: list (A * B)) l',
+  l *=* l' ->
+  from_list (map fst_ l) = from_list (map fst_ l').
+intros A B; induction l; intros.
+apply permut_nil_eq in H; subst; auto.
+assert (a :: l *=* l') by auto;
+apply permut_split_head in H; destruct H as (hd', (tl', H)); subst.
+assert (from_list (map fst_ l) = from_list (map fst_ (hd' ++ tl'))).
+  apply IHl; apply permut_cons_inv with (a:=a); rewrite H0; permut_simpl.
+  destruct a; rew_map; simpl; rewrite from_list_cons; rewrite H.
+  rewrite map_app; repeat rewrite from_list_app; rewrite from_list_cons.
+  rewrite union_comm_assoc; auto.
+Qed.
+
+Lemma from_list_Mem:
+forall A U (x:A), Mem x U <-> x \in from_list U.
+intro A; induction U; split; intros.
+rewrite Mem_nil_eq in H; contradiction.
+rewrite from_list_nil in H; apply notin_empty in H; contradiction.
+rewrite Mem_cons_eq in H; destruct H; subst; rewrite from_list_cons;
+rewrite in_union.
+  left; rewrite in_singleton; auto.
+  right; eapply IHU; auto.
+rewrite Mem_cons_eq; rewrite from_list_cons in H; rewrite in_union in H;
+destruct H; subst.
+  left; rewrite in_singleton in H; subst; auto.
+  right; eapply IHU; auto.
+Qed.
